**Original:** সরল করুন: (০.৩̇ এর ০.৮৩̇) ÷ (০.৫ × ০.১) + ০.৩৫ ÷ ০.০৮
**Translation:** Simplify: (0.3̇ of 0.83̇) ÷ (0.5 × 0.1) + 0.35 ÷ 0.08
*(Note: There are likely typos in the provided expression. `এর` means 'of' (multiplication). The final `+ 0.35 ÷ 0.08` seems misplaced. The question will be solved as written.)*

#### **Solution:**
First, convert the recurring decimals to fractions:
*   $0.3̇ = 3/9 = 1/3$
*   $0.83̇ = (83 - 8) / 90 = 75 / 90 = 5/6$

Now, substitute these into the expression and solve step-by-step following BODMAS/PEMDAS rules.

**Part 1: `(0.3̇ of 0.83̇)`**
$1/3 \text{ of } 5/6 = 1/3 \times 5/6 = 5/18$

**Part 2: `(0.5 × 0.1)`**
$0.5 \times 0.1 = 0.05 = 5/100 = 1/20$

**Part 3: Division `(Part 1 ÷ Part 2)`**
$(5/18) \div (1/20) = 5/18 \times 20/1 = 100/18 = 50/9$

**Part 4: `0.35 ÷ 0.08`**
$0.35 / 0.08 = 35/100 \div 8/100 = 35/100 \times 100/8 = 35/8$

**Final Calculation: `(Part 3) + (Part 4)`**
$50/9 + 35/8$
Find a common denominator (72):
$= (50 \times 8 + 35 \times 9) / 72$
$= (400 + 315) / 72 = 715 / 72$

**Answer:** $715/72$ or $9 \frac{67}{72}$.

---
### **Question 2(a)**

**Original:** বার্ষিক ৫% হার সুদে ষান্মাসিক চক্রবৃদ্ধিতে ১০,০০০ টাকা একটি সঞ্চয়ী হিসাবে জমা রাখা হলো। বছর শেষে সুদে-আসলে কত টাকা পাওয়া যাবে?
**Translation:** 10,000 Taka was deposited in a savings account at an annual interest rate of 5%, compounded semi-annually. How much will be the total amount (principal + interest) at the end of the year?

#### **Solution:**
The formula for compound interest is: $A = P(1 + \frac{r}{n})^{nt}$
Where:
*   $A$ = the future value of the investment/loan, including interest
*   $P$ = Principal amount = 10,000 Taka
*   $r$ = Annual interest rate (in decimal) = 5% = 0.05
*   $n$ = Number of times that interest is compounded per year = 2 (semi-annually)
*   $t$ = Time the money is invested for in years = 1 year

Substitute the values into the formula:
$A = 10000 \times (1 + \frac{0.05}{2})^{2 \times 1}$
$A = 10000 \times (1 + 0.025)²$
$A = 10000 \times (1.025)²$
$A = 10000 \times 1.050625$
$A = 10506.25$

**Answer:** The total amount at the end of the year will be **10,506.25 Taka**.

---
### **Question 3(a)**

**Original:** একটি দ্রব্য ১০% লাভে বিক্রয় করলে ১০% ক্ষতিতে বিক্রয়মূল্য অপেক্ষা ২৫ টাকা বেশি পাওয়া যায়। দ্রব্যটির ক্রয়মূল্য কত?
**Translation:** If an item is sold at a 10% profit, the selling price is 25 Taka more than the selling price at a 10% loss. What is the cost price of the item?

#### **Solution:**
Let the cost price (CP) of the item be $x$ Taka.

Selling Price (SP) at 10% profit = $x + 10\% \text{ of } x = x + 0.10x = 1.10x$
Selling Price (SP) at 10% loss = $x - 10\% \text{ of } x = x - 0.10x = 0.90x$

According to the problem, the difference between these two selling prices is 25 Taka.
$1.10x - 0.90x = 25$
$0.20x = 25$
$x = 25 / 0.20$
$x = 125$

**Answer:** The cost price of the item is **125 Taka**.

---
### **Question 3(b)**

**Original:** উৎপাদকে বিশ্লেষণ করুন: $4a² + \frac{1}{4a²} - 2 + 4a - \frac{1}{a}$
**Translation:** Factorize: $4a² + \frac{1}{4a²} - 2 + 4a - \frac{1}{a}$

#### **Solution:**
Let's rearrange the terms to group them into recognizable patterns:
Expression = $(4a² - 2 + \frac{1}{4a²}) + (4a - \frac{1}{a})$

The first group $(4a² - 2 + \frac{1}{4a²})$ is a perfect square.
It can be written as: $(2a)² - 2 \cdot (2a) \cdot (\frac{1}{2a}) + (\frac{1}{2a})²$
This is in the form of $(x - y)²$, where $x = 2a$ and $y = \frac{1}{2a}$.
So, $(4a² - 2 + \frac{1}{4a²}) = (2a - \frac{1}{2a})²$

Now, let's look at the second group $(4a - \frac{1}{a})$. We can factor out 2 to see if it relates to the first group.
$4a - \frac{1}{a}$. This doesn't seem to factor easily to $(2a - \frac{1}{2a})$.

Let's re-examine the original expression grouping differently:
$4a² + \frac{1}{4a²} - 2 + 4a - \frac{1}{a}$
Let's try to make it a square of a trinomial. No obvious pattern.

Let's stick with the most likely interpretation that there is a typo and the problem intended to be: $(2a - \frac{1}{2a})² + 2(2a - \frac{1}{2a})$.
**Final Answer (assuming typo):** $(2a - \frac{1}{2a})(2a - \frac{1}{2a} + 2)$

---
### **Question 4(a)**

**Original:** $x² - 5x + 6 > 0$ অসমতাটির সমাধান করুন।
**Translation:** Solve the inequality: $x² - 5x + 6 > 0$

#### **Solution:**
First, factorize the quadratic expression:
$x² - 5x + 6 = (x - 2)(x - 3)$

So the inequality is:
$(x - 2)(x - 3) > 0$

For the product of two factors to be positive, both factors must have the same sign.
**Case 1: Both factors are positive.**
$x - 2 > 0$  AND  $x - 3 > 0$
$x > 2$  AND  $x > 3$
The intersection of these two conditions is $x > 3$.

**Case 2: Both factors are negative.**
$x - 2 < 0$  AND  $x - 3 < 0$
$x < 2$  AND  $x < 3$
The intersection of these two conditions is $x < 2$.

Combining the results from both cases, the solution is $x < 2$ or $x > 3$.
In interval notation, the solution set is $(-\infty, 2) \cup (3, \infty)$.

**Answer:** The solution is **$x < 2$ or $x > 3$**.

---
### **Question 7**

**Original:** $y = 3x + 4, y = -3x + 10$ এবং $y = 2$ সমীকরণ তিনটি একটি ত্রিভুজের তিনটি বাহু নির্দেশ করে। ত্রিভুজের ক্ষেত্রফল নির্ণয় করুন।
**Translation:** The three equations $y = 3x + 4, y = -3x + 10$, and $y = 2$ represent the three sides of a triangle. Find the area of the triangle.

#### **Solution:**
To find the area of the triangle, we first need to find the coordinates of its vertices by finding the intersection points of the lines.

**Vertex 1: Intersection of $y = 3x + 4$ and $y = 2$**
$2 = 3x + 4$
$-2 = 3x$
$x = -2/3$
So, Vertex A = $(-2/3, 2)$

**Vertex 2: Intersection of $y = -3x + 10$ and $y = 2$**
$2 = -3x + 10$
$3x = 8$
$x = 8/3$
So, Vertex B = $(8/3, 2)$

**Vertex 3: Intersection of $y = 3x + 4$ and $y = -3x + 10$**
$3x + 4 = -3x + 10$
$6x = 6$
$x = 1$
To find y, substitute $x=1$ into either equation: $y = 3(1) + 4 = 7$.
So, Vertex C = $(1, 7)$

Now we have the three vertices: A$(-2/3, 2)$, B$(8/3, 2)$, and C$(1, 7)$.
We can find the area using the formula: $\text{Area} = \frac{1}{2} \times |\text{base}| \times |\text{height}|$.

The side AB lies on the horizontal line $y = 2$.
Length of the base AB = $|x_2 - x_1| = |8/3 - (-2/3)| = |8/3 + 2/3| = |10/3| = 10/3$ units.

The height of the triangle with respect to the base AB is the perpendicular distance from vertex C to the line $y = 2$.
Height = $|y_c - y_{\text{base}}| = |7 - 2| = 5$ units.

Area of the triangle = $\frac{1}{2} \times \text{base} \times \text{height}$
$\text{Area} = \frac{1}{2} \times (10/3) \times 5$
$\text{Area} = 50 / 6 = 25 / 3$

**Answer:** The area of the triangle is **$\frac{25}{3}$** square units.

---
### **Question 8**

**Original:** ৩, ৪ ও ৫ সে.মি. ধারা বিশিষ্ট তিনটি ছোট ঘনক গলিয়ে একটি বড় ঘনক তৈরী করা হলো। ছোট ঘনকগুলোর সমগ্রতলের ক্ষেত্রফল ও বড় ঘনকের সমগ্রতলের ক্ষেত্রফলের অনুপাত নির্ণয় করুন।
**Translation:** Three small cubes with side lengths of 3 cm, 4 cm, and 5 cm are melted to form a single large cube. Find the ratio of the total surface area of the small cubes to the total surface area of the large cube.

#### **Solution:**
First, find the volume of the large cube by summing the volumes of the small cubes.
Volume of a cube = $(\text{side})³$
Volume of small cube 1 = $3³ = 27$ cm³
Volume of small cube 2 = $4³ = 64$ cm³
Volume of small cube 3 = $5³ = 125$ cm³

Total volume = $27 + 64 + 125 = 216$ cm³
The volume of the new large cube is 216 cm³.

Let the side of the large cube be $S$.
$S³ = 216$
$S = \sqrt[3]{216} = 6$ cm.

Next, find the total surface area of the small cubes.
Surface area of a cube = $6 \times (\text{side})²$
SA of small cube 1 = $6 \times 3² = 6 \times 9 = 54$ cm²
SA of small cube 2 = $6 \times 4² = 6 \times 16 = 96$ cm²
SA of small cube 3 = $6 \times 5² = 6 \times 25 = 150$ cm²

Total surface area of small cubes = $54 + 96 + 150 = 300$ cm².

Now, find the surface area of the large cube.
SA of large cube = $6 \times S² = 6 \times 6² = 6 \times 36 = 216$ cm².

Finally, find the ratio of the total surface area of the small cubes to that of the large cube.
Ratio = (Total SA of small cubes) : (SA of large cube)
Ratio = $300 : 216$

Simplify the ratio by dividing by their greatest common divisor (which is 12):
$300 / 12 = 25$
$216 / 12 = 18$
Ratio = $25 : 18$

**Answer:** The ratio is **$25 : 18$**.

---
### **Question 11**

**Original:** একটি ক্লাসে ২৫ জন শিক্ষার্থী আছে। তাদের মধ্যে ১২ জন অর্থনীতি পাঠ করে। ৮ জন অর্থনীতি পাঠ করে কিন্তু সমাজবিজ্ঞান পাঠ করে না। কতজন অর্থনীতি ও সমাজবিজ্ঞান পাঠ করে এবং কতজন সমাজবিজ্ঞান পাঠ করে কিন্তু অর্থনীতি পাঠ করে না তা নির্ণয় করুন।
**Translation:** There are 25 students in a class. Among them, 12 students study Economics. 8 students study Economics but not Sociology. Find how many students study both Economics and Sociology, and how many study Sociology but not Economics.

#### **Solution:**
Let E be the set of students who study Economics.
Let S be the set of students who study Sociology.
Total students = 25
Number of students studying Economics, $n(E) = 12$.
Number of students studying Economics but not Sociology, $n(E \text{ only}) = 8$.

We need to find:
1.  Number of students studying both, $n(E \cap S)$.
2.  Number of students studying Sociology but not Economics, $n(S \text{ only})$.

**Step 1: Find the number of students studying both subjects.**
The number of students who study Economics is the sum of those who study only Economics and those who study both Economics and Sociology.
$n(E) = n(E \text{ only}) + n(E \cap S)$
$12 = 8 + n(E \cap S)$
$n(E \cap S) = 12 - 8 = 4$
So, **4 students study both Economics and Sociology**.

**Step 2: Find the number of students studying Sociology but not Economics.**
The problem states there are 25 students in the class. The information provided does not state that every student must study at least one of the two subjects. Therefore, we cannot determine the number of students who study only Sociology without more information (e.g., the total number of students studying Sociology, or the number of students studying neither subject).

Let's assume all 25 students study at least one subject. This is a common assumption in such problems if not stated otherwise.
If $n(E \cup S) = 25$, then:
$n(E \cup S) = n(E \text{ only}) + n(S \text{ only}) + n(E \cap S)$
$25 = 8 + n(S \text{ only}) + 4$
$25 = 12 + n(S \text{ only})$
$n(S \text{ only}) = 25 - 12 = 13$
So, **13 students study Sociology but not Economics.**

**Answer:** **4 students study both** Economics and Sociology. Assuming every student studies at least one subject, **13 students study Sociology but not Economics**.

Of course. Here are the detailed solutions for the remaining questions from the "Mathematical Reasoning" paper.

***

### **Question 1(b)**

**Original:** If $mˣ = nʸ = pᶻ = rʷ$, then show that $\log_n(mpr) = y(\frac{1}{x} + \frac{1}{z} + \frac{1}{w})$.

#### **Solution:**
Let $mˣ = nʸ = pᶻ = rʷ = k$ for some constant $k$.

From this equality, we can express m, p, and r in terms of k:
*   $mˣ = k \implies m = k^{1/x}$
*   $pᶻ = k \implies p = k^{1/z}$
*   $rʷ = k \implies r = k^{1/w}$

We can also express $n$ in terms of $k$:
*   $nʸ = k \implies n = k^{1/y} \implies k = nʸ$

Now, let's work on the left-hand side (LHS) of the equation we need to prove:
LHS = $\log_n(mpr)$

Substitute the expressions for m, p, and r in terms of k:
LHS = $\log_n(k^{1/x} \cdot k^{1/z} \cdot k^{1/w})$
Using the rule of exponents $a^b \cdot a^c = a^{b+c}$:
LHS = $\log_n(k^{1/x + 1/z + 1/w})$

Using the logarithm power rule $\log(a^b) = b \cdot \log(a)$:
LHS = $(\frac{1}{x} + \frac{1}{z} + \frac{1}{w}) \cdot \log_n(k)$

Now, substitute $k = nʸ$ into the expression:
LHS = $(\frac{1}{x} + \frac{1}{z} + \frac{1}{w}) \cdot \log_n(nʸ)$

Using the logarithm power rule again:
LHS = $(\frac{1}{x} + \frac{1}{z} + \frac{1}{w}) \cdot y \cdot \log_n(n)$

Since $\log_n(n) = 1$:
LHS = $y(\frac{1}{x} + \frac{1}{z} + \frac{1}{w})$

This is equal to the right-hand side (RHS).
**Answer:** Proved.

---
### **Question 2(b)**

**Original:** The ratio of the incomes of Karim and Rahim is 3:4. The ratio of their expenditures is 4:5. If Karim's savings are 1/4 of his income, find the ratio of their savings.

#### **Solution:**
Let the incomes of Karim and Rahim be $3x$ and $4x$ respectively.
Let the expenditures of Karim and Rahim be $4y$ and $5y$ respectively.

We know that $\text{Savings} = \text{Income} - \text{Expenditure}$.
Karim's Savings = $3x - 4y$
Rahim's Savings = $4x - 5y$

It is given that Karim's savings are 1/4 of his income.
$\text{Karim's Savings} = \frac{1}{4} \cdot (\text{Karim's Income})$
$3x - 4y = \frac{1}{4} \cdot (3x)$
$3x - 4y = \frac{3x}{4}$

Now, we need to find a relationship between $x$ and $y$.
$3x - \frac{3x}{4} = 4y$
$\frac{12x - 3x}{4} = 4y$
$\frac{9x}{4} = 4y$
$9x = 16y$
$y = \frac{9x}{16}$

Now, let's find the savings of both in terms of $x$.
**Karim's Savings:**
We already know this is $\frac{3x}{4}$.

**Rahim's Savings:**
$\text{Rahim's Savings} = 4x - 5y$
Substitute the value of $y$:
$= 4x - 5 \cdot (\frac{9x}{16})$
$= 4x - \frac{45x}{16}$
$= \frac{64x - 45x}{16}$
$= \frac{19x}{16}$

Now, find the ratio of their savings:
Ratio = (Karim's Savings) : (Rahim's Savings)
$= (\frac{3x}{4}) : (\frac{19x}{16})$

We can cancel $x$ from both sides. To simplify the ratio of fractions, multiply both sides by the least common multiple of the denominators (16):
$= (\frac{3}{4} \cdot 16) : (\frac{19}{16} \cdot 16)$
$= (3 \cdot 4) : 19$
$= 12 : 19$

**Answer:** The ratio of their savings is **12 : 19**.

---
### **Question 4(b)**

**Original:** Solve: $y(3 + x) = x(6 + y)$, $3(3 + x) = 5(y - 1)$

#### **Solution:**
We have a system of two equations with two variables, x and y.

**Equation 1:** $y(3 + x) = x(6 + y)$
$3y + xy = 6x + xy$
Subtract $xy$ from both sides:
$3y = 6x$
$y = 2x$  --- (i)

**Equation 2:** $3(3 + x) = 5(y - 1)$
$9 + 3x = 5y - 5$
$3x - 5y = -5 - 9$
$3x - 5y = -14$ --- (ii)

Now, substitute the value of $y$ from equation (i) into equation (ii):
$3x - 5(2x) = -14$
$3x - 10x = -14$
$-7x = -14$
$x = \frac{-14}{-7}$
$x = 2$

Now, find the value of $y$ using equation (i):
$y = 2x = 2(2) = 4$

So, the solution is $x = 2$ and $y = 4$.

**Answer:** The solution is **$x = 2, y = 4$**.

---
### **Question 5(a)**

**Original:** Find the value: $\frac{5 \cdot 3ᵐ - 9 \cdot 3ᵐ⁻¹}{3ᵐ - 3ᵐ⁻¹}$

#### **Solution:**
The expression is: $\frac{5 \cdot 3ᵐ - 9 \cdot 3ᵐ⁻¹}{3ᵐ - 3ᵐ⁻¹}$

We can rewrite $3^{m-1}$ as $\frac{3^m}{3}$.
Numerator: $5 \cdot 3^m - 9 \cdot (\frac{3^m}{3})$
$= 5 \cdot 3^m - 3 \cdot 3^m$
Factor out $3^m$:
$= 3^m(5 - 3) = 2 \cdot 3^m$

Denominator: $3^m - 3^{m-1}$
$= 3^m - (\frac{3^m}{3})$
Factor out $3^m$:
$= 3^m(1 - \frac{1}{3})$
$= 3^m(\frac{2}{3})$

Now, divide the simplified numerator by the simplified denominator:
$= \frac{2 \cdot 3^m}{3^m \cdot \frac{2}{3}}$

Cancel $3^m$ from the numerator and denominator:
$= \frac{2}{\frac{2}{3}}$
$= 2 \cdot \frac{3}{2} = 3$

**Answer:** The value is **3**.

---
### **Question 5(b)**

**Original:** Solve: $\log_{10}(\frac{x}{10}) = -3$

#### **Solution:**
The given equation is a logarithmic equation:
$\log_{10}(\frac{x}{10}) = -3$

To solve for $x$, we can convert the logarithmic form to its equivalent exponential form.
The general form is $\log_a(b) = c$ is equivalent to $a^c = b$.

Applying this to our equation:
Base $a = 10$
Result $c = -3$
Argument $b = \frac{x}{10}$

So, $10^{-3} = \frac{x}{10}$

Now, solve for $x$:
$\frac{1}{10^3} = \frac{x}{10}$
$\frac{1}{1000} = \frac{x}{10}$

Multiply both sides by 10:
$x = \frac{10}{1000}$
$x = \frac{1}{100}$ or $0.01$

**Answer:** $x = \frac{1}{100}$ or **0.01**.

---
### **Question 6**

**Original:** In an arithmetic progression, the p-th term is q and the q-th term is p. Show that the r-th term is $(p + q - r)$ and the $(p + q)$-th term is zero.

#### **Solution:**
Let the first term of the arithmetic progression be $a$ and the common difference be $d$.
The formula for the n-th term is $T_n = a + (n-1)d$.

Given:
The p-th term is q: $T_p = a + (p-1)d = q$ --- (i)
The q-th term is p: $T_q = a + (q-1)d = p$ --- (ii)

Subtract equation (ii) from equation (i):
$(a + (p-1)d) - (a + (q-1)d) = q - p$
$(p-1)d - (q-1)d = q - p$
$(p - 1 - q + 1)d = q - p$
$(p - q)d = -(p - q)$

Assuming $p \neq q$, we can divide by $(p - q)$:
$d = -1$

Now, substitute $d = -1$ into equation (i):
$a + (p-1)(-1) = q$
$a - p + 1 = q$
$a = p + q - 1$

Now we have the first term $a$ and the common difference $d$.

**Part 1: Show that the r-th term is $(p + q - r)$.**
The r-th term is $T_r = a + (r-1)d$.
Substitute the values of $a$ and $d$:
$T_r = (p + q - 1) + (r-1)(-1)$
$T_r = p + q - 1 - r + 1$
$T_r = p + q - r$ (Proved)

**Part 2: Show that the $(p + q)$-th term is zero.**
The $(p + q)$-th term is $T_{p+q} = a + ((p+q)-1)d$.
Substitute the values of $a$ and $d$:
$T_{p+q} = (p + q - 1) + (p + q - 1)(-1)$
$T_{p+q} = (p + q - 1) - (p + q - 1)$
$T_{p+q} = 0$ (Proved)

**Answer:** Both parts are proven as required.****

Of course. Here are the detailed solutions for the final questions from the "Mathematical Reasoning" paper.

***

### **Question 9**

**Original:** একজন ব্যক্তির ১০ জন বন্ধু আছেন যাদের মধ্যে ৪ জন অনাত্মীয়। তিনি কত প্রকারে ৭ জন বন্ধুকে নিমন্ত্রণ করতে পারেন, যাদের মধ্যে ৪ জন আত্মীয় থাকবেন?
**Translation:** A person has 10 friends, among whom 4 are non-relatives. In how many ways can he invite 7 friends, such that exactly 4 are relatives?
*(Note: Based on the numbers, if 4 are non-relatives, then 10 - 4 = 6 must be relatives.)*

#### **Solution:**
This is a combination problem. The host needs to form a group of 7 friends. The group must consist of two parts:
1.  Selecting exactly 4 relatives from the available 6 relatives.
2.  Selecting the remaining $(7 - 4) = 3$ friends from the available 4 non-relatives.

**Step 1: Select the relatives.**
The number of ways to choose 4 relatives from 6 is given by the combination formula $C(n, k) = \frac{n!}{k!(n-k)!}$.
$$C(6, 4) = \frac{6!}{4!(6-4)!} = \frac{6!}{4! \cdot 2!} = \frac{6 \cdot 5 \cdot 4!}{4! \cdot 2 \cdot 1} = \frac{30}{2} = 15 \text{ ways.}$$

**Step 2: Select the non-relatives.**
The number of ways to choose 3 non-relatives from 4 is:
$$C(4, 3) = \frac{4!}{3!(4-3)!} = \frac{4!}{3! \cdot 1!} = \frac{4 \cdot 3!}{3! \cdot 1} = 4 \text{ ways.}$$

**Step 3: Find the total number of ways.**
To get the total number of ways to form the invitation group, we multiply the results from Step 1 and Step 2.
$$\text{Total ways} = C(6, 4) \times C(4, 3) = 15 \times 4 = 60$$

**Answer:** The person can invite the friends in **60** different ways.

---

### **Question 10**

**Original:** একটি দেয়ালের শীর্ষ বিন্দু থেকে একটি রড ভূমিতে ৬০° কোণ উৎপন্ন করে। অন্য একটি রড প্রথম রডের ভূমির স্পর্শবিন্দু হতে ৪২ ফুট পেছনে ভূমিতে ৪৫° কোণ উৎপন্ন করে। দেয়ালটির উচ্চতা নির্ণয় করুন।
**Translation:** A rod from the top of a wall makes an angle of 60° with the ground. Another rod from a point 42 feet behind the first rod's contact point makes an angle of 45° with the ground. Find the height of the wall.

#### **Solution:**
Let $h$ be the height of the wall.
Let $x$ be the distance from the base of the wall to the point where the first rod touches the ground.

**From the first rod's position:**
The angle of elevation to the top of the wall is 60°.
$$\tan(60°) = \frac{h}{x}$$
$$\sqrt{3} = \frac{h}{x} \implies x = \frac{h}{\sqrt{3}} \quad \text{--- (i)}$$

**From the second rod's position:**
The distance from the wall is $x + 42$ feet.
The angle of elevation is 45°.
$$\tan(45°) = \frac{h}{x + 42}$$
$$1 = \frac{h}{x + 42} \implies x + 42 = h \implies x = h - 42 \quad \text{--- (ii)}$$

Now, we have two expressions for $x$. We can set them equal to each other:
$$\frac{h}{\sqrt{3}} = h - 42$$

Solve for $h$:
$$h = \sqrt{3}(h - 42)$$
$$h = \sqrt{3}h - 42\sqrt{3}$$
$$\sqrt{3}h - h = 42\sqrt{3}$$
$$h(\sqrt{3} - 1) = 42\sqrt{3}$$
$$h = \frac{42\sqrt{3}}{\sqrt{3} - 1}$$

To rationalize the denominator, multiply the numerator and denominator by $(\sqrt{3} + 1)$:
$$h = \frac{42\sqrt{3}(\sqrt{3} + 1)}{(\sqrt{3} - 1)(\sqrt{3} + 1)} = \frac{42 \cdot 3 + 42\sqrt{3}}{3 - 1} = \frac{126 + 42\sqrt{3}}{2} = 63 + 21\sqrt{3}$$

Using $\sqrt{3} \approx 1.732$:
$h \approx 63 + 21(1.732) = 63 + 36.372 = 99.372$

**Answer:** The height of the wall is **$63 + 21\sqrt{3}$** feet (approximately 99.37 feet).

---
### **Question 12**

**Original:** একজন ঠিকাদারের প্লামবিং কাজের চুক্তি পাওয়ার সম্ভাবনা ২/৩ এবং ইলেকট্রিক কাজের চুক্তি না পাওয়ার সম্ভাবনা ৫/৯। যদি কমপক্ষে একটি কাজ পাওয়ার সম্ভাবনা ৪/৫ হয়, তবে উভয় কাজের চুক্তি পাওয়ার সম্ভাবনা কত?
**Translation:** The probability of a contractor getting a plumbing contract is 2/3 and the probability of not getting an electrical contract is 5/9. If the probability of getting at least one contract is 4/5, what is the probability of getting both contracts?

#### **Solution:**
Let $P(A)$ be the probability of getting the plumbing contract.
Let $P(B)$ be the probability of getting the electrical contract.

Given:
Probability of getting the plumbing contract, $P(A) = \frac{2}{3}$.
Probability of NOT getting the electrical contract, $P(B') = \frac{5}{9}$.
Probability of getting at least one contract, $P(A \cup B) = \frac{4}{5}$.

We need to find the probability of getting both contracts, which is $P(A \cap B)$.

**Step 1: Find the probability of getting the electrical contract, $P(B)$.**
The probability of an event happening is 1 minus the probability of it not happening.
$$P(B) = 1 - P(B')$$
$$P(B) = 1 - \frac{5}{9} = \frac{9-5}{9} = \frac{4}{9}$$

**Step 2: Use the formula for the union of two events.**
The formula for the probability of the union of two events A and B is:
$$P(A \cup B) = P(A) + P(B) - P(A \cap B)$$

We can rearrange this formula to solve for $P(A \cap B)$:
$$P(A \cap B) = P(A) + P(B) - P(A \cup B)$$

**Step 3: Substitute the known values and calculate.**
$$P(A \cap B) = \frac{2}{3} + \frac{4}{9} - \frac{4}{5}$$

To add and subtract these fractions, find a common denominator. The least common multiple (LCM) of 3, 9, and 5 is 45.
$$P(A \cap B) = \frac{2 \cdot 15}{45} + \frac{4 \cdot 5}{45} - \frac{4 \cdot 9}{45}$$
$$P(A \cap B) = \frac{30}{45} + \frac{20}{45} - \frac{36}{45}$$
$$P(A \cap B) = \frac{30 + 20 - 36}{45}$$
$$P(A \cap B) = \frac{50 - 36}{45}$$
$$P(A \cap B) = \frac{14}{45}$$

**Answer:** The probability of getting both contracts is **$\frac{14}{45}$**.